toList + pruebas auxiliares

BinomialHeap.fst
@@ -1,10 +1,12 @@
 module BinomialHeap
 
 open FStar.List.Tot
+open FStar.Math.Lib
+open FStar.Calc
 
-type node0 = | N of int & int & list node0 // rank, data, children
+type node0 = | N of nat & int & list node0 // rank, data, children
 
-let rank (tree : node0) : int =
+let rank (tree : node0) : nat =
   let N (r,_,_) = tree in
   r
 
@@ -24,18 +26,26 @@ let link (tree1 : node0) (tree2 : node0{rank tree2 = rank tree1}) : node0 =
                                     then N (r + 1, k1, tree2 :: c1)
                                     else N (r + 1, k2, tree1 :: c2)
 
-let rec all_nodes (bound : 'a) (f: (x:node0{x << bound}) -> bool) (l : list node0{l << bound}) : bool =
+let rec all_nodes (#a:Type) (#b: Type) (bound : a) (f: (x:node0{x << bound}) -> b) (op: b -> b -> b) (e: b) (l: list node0{l << bound}) : b = 
   match l with
-  | [] -> true
-  | x::xs' -> f x && all_nodes bound f xs'
+    | [] -> e
+    | x::xs -> op (f x) (all_nodes bound f op e xs)
 
-let rec all_le (x: int) (tree: node0) : bool =
+let rec all_le0 (x: int) (tree: node0) : bool =
   match tree with
-  | N (r, k, c) -> k <= x && all_nodes tree (all_le x) c
+  | N (r, k, c) -> k <= x && all_le x c
+and all_le (x: int) (bh: list node0) : bool =
+  match bh with
+    | [] -> true
+    | h::hs -> all_le0 x h && all_le x hs
 
-let rec is_heap (tree: node0) : bool =
+let rec is_heap0 (tree: node0) : bool =
   match tree with
-  | N (r, k, c) -> all_le k tree && all_nodes tree is_heap c
+  | N (r, k, c) -> all_le0 k tree && is_heap c
+and is_heap (bh: list node0) : bool =
+  match bh with
+    | [] -> true
+    | h::hs -> is_heap0 h && is_heap hs
 
 let rec incr_rank (hs : list node0) : prop =
   match hs with
@@ -43,16 +53,24 @@ let rec incr_rank (hs : list node0) : prop =
   | [_] -> True
   | h1::h2::hs' -> rank h1 < rank h2 /\ incr_rank (h2::hs')
 
-type heap = list node0
+let rec number_nodes0 (tree: node0) : nat =
+  match tree with
+  | N (_, _, c) -> 1 + number_nodes c
+and number_nodes (bh: list node0) : nat = 
+  match bh with
+    | [] -> 0
+    | h::hs -> number_nodes0 h + number_nodes hs
 
-let emptyHeap : heap = []
+type bheap = list node0
 
-let isEmptyHeap (h: heap) : bool =
+let emptyHeap : bheap = []
+
+let isEmptyHeap (h: bheap) : bool =
   match h with
   | [] -> true
   | _ -> false
 
-let rec insertTree (t: node0) (bh: heap) : Tot heap (decreases (length bh))=
+let rec insertTree (t: node0) (bh: bheap) : Tot bheap (decreases (length bh))=
   match bh with
   | [] -> [t]
   | h::hs -> if rank t < rank h
@@ -61,10 +79,10 @@ let rec insertTree (t: node0) (bh: heap) : Tot heap (decreases (length bh))=
                   then insertTree (link t h) hs
                   else h :: insertTree t hs
 
-let insert (x: int) (h: heap) : heap =
+let insert (x: int) (h: bheap) : bheap =
   insertTree (singleton x) h
 
-let rec merge (bh1: heap) (bh2: heap) : heap =
+let rec merge (bh1: bheap) (bh2: bheap) : bheap =
   match bh1, bh2 with
   | [], _ -> bh2
   | _, [] -> bh1
@@ -74,7 +92,7 @@ let rec merge (bh1: heap) (bh2: heap) : heap =
                              then h2 :: merge bh1 hs2
                              else insertTree (link h1 h2) (merge hs1 hs2)
 
-let rec removeMinTree (bh: heap{Cons? bh}) : node0 & heap =
+let rec removeMinTree (bh: bheap{Cons? bh}) : (node0 & bheap)  =
   match bh with
   | [h] -> (h, [])
   | h::hs -> let m, hs' = removeMinTree hs in
@@ -82,17 +100,83 @@ let rec removeMinTree (bh: heap{Cons? bh}) : node0 & heap =
              then (h, hs)
              else (m, h::hs')
 
-let findMin (bh: heap{Cons? bh}) : int =
+// let lemma_removeMinTree (bh : bheap{Cons? bh})
+//   : Lemma (let (t, bh') = removeMinTree bh in
+//            is_perm (t :: bh') bh)
+//   = ...
+
+let rec lemma_removeMinTree_size (bh : bheap{Cons? bh})
+  : Lemma (number_nodes bh == number_nodes (snd (removeMinTree bh)) + number_nodes0 (fst (removeMinTree bh)))
+  = match bh with
+    | [h] -> ()
+    | h::hs -> lemma_removeMinTree_size hs
+
+let findMin (bh: bheap{Cons? bh}) : int =
   let m, _ = removeMinTree bh in root m
 
-let rev (#a:Type) (xs : list a) : list a =
-  let rec go (acc xs : list a) : Tot (list a) (decreases xs)=
-    match xs with
-    | [] -> acc
-    | x::xs -> go (x::acc) xs
-  in
-  go [] xs
+let rec rev_go #a (acc xs : list a) : Tot (list a) (decreases xs)=
+  match xs with
+  | [] -> acc
+  | x::xs -> rev_go (x::acc) xs
 
-let deleteMin (bh: heap{Cons? bh}) : heap =
+let rev (#a:Type) (xs : list a) : list a =
+  rev_go [] xs
+
+let extractMin (bh: bheap{Cons? bh}) : int & bheap =
   let m, hs = removeMinTree bh in
-  merge (rev (children m)) hs
+  root m, merge (rev (children m)) hs
+
+let rec lemma_rev_go_number_nodes (acc ts : list node0)
+  : Lemma (ensures number_nodes acc + number_nodes ts == number_nodes (rev_go acc ts))
+          (decreases ts)
+  =  match ts with
+     | [] -> ()
+     | t::ts -> lemma_rev_go_number_nodes (t::acc) ts
+
+let lemma_rev_number_nodes (ts : list node0)
+  : Lemma (number_nodes ts == number_nodes (rev ts))
+          [SMTPat (number_nodes (rev ts))]
+  = lemma_rev_go_number_nodes [] ts
+
+let deleteMin_size (bh: bheap{Cons? bh})
+  : Lemma (number_nodes (snd (extractMin bh)) == number_nodes bh - 1)
+= 
+  let m, hs = removeMinTree bh in
+  calc (==) {
+    number_nodes (snd (extractMin bh));
+    == {}
+    number_nodes (merge (rev (children m)) hs);
+    == { admit() } (* demostrar que size(merge a b) = size a + size b *)
+    number_nodes (rev (children m)) + number_nodes hs;
+    // == { } // lemma_rev_number_nodes (children m) }
+    // number_nodes (children m) + number_nodes hs;
+    // == { } // children_size m }
+    // (number_nodes0 m - 1) + number_nodes hs;
+    // == {}
+    // (number_nodes0 m + number_nodes hs) - 1;
+    == { lemma_removeMinTree_size bh }
+    number_nodes bh - 1;
+  }
+
+let rec toList (bh: bheap) : Tot (list int) (decreases (number_nodes bh))=
+  match bh with
+    | [] -> []
+    | _ -> let m, bh' = extractMin bh in
+           deleteMin_size bh;
+           m :: toList bh'
+
+let models (bh : bheap) (xs : list int) : prop =
+  toList bh == xs
+
+// val insert_ok (x:int) (bh : bheap) (xs : list int)
+//   : Lemma (requires models bh xs)
+//           (ensures models (insert x bh) (x :: xs))
+
+// val peek_ok (bh : bheap) (x:int) (xs : list int)
+//   : Lemma (requires models bh (x::xs))
+//           (ensures peek bh == x)
+
+let rec fromList (l: list int) : bheap =
+  match l with
+    | [] -> []
+    | x::xs -> insert x (fromList xs)
